Add macros for loading flattened structs

src/go_lang/struct.v
@@ -14,18 +14,15 @@ Record descriptor :=
 Section go_lang.
   Context `{ffi_sem: ext_semantics}.
 
-  Definition Var' s : @expr ext := Var s.
-  Local Coercion Var' : string >-> expr.
-
-Fixpoint getField_e (f0: string) (rev_fields: list (string*ty)): expr :=
+Fixpoint getField_e (f0: string) (rev_fields: list (string*ty)) (se: expr): expr :=
   match rev_fields with
   | [] => LitV LitUnit
-  | [f] => if String.eqb (fst f) f0 then "v" else #()
-  | f::fs => if String.eqb (fst f) f0 then Snd "v" else Fst (getField_e f0 fs)
+  | [f] => if String.eqb (fst f) f0 then se else #()
+  | f::fs => if String.eqb (fst f) f0 then Snd se else Fst (getField_e f0 fs se)
   end.
 
 Definition getField (d:descriptor) f : val :=
-  λ: "v", getField_e f (rev d.(fields)).
+  λ: "v", getField_e f (rev d.(fields)) (Var "v").
 
 Fixpoint assocl_lookup {A} (field_vals: list (string * A)) (f0: string) : option A :=
   match field_vals with
@@ -64,6 +61,34 @@ Fixpoint struct_ty_prod (rev_fields: list (string*ty)) : ty :=
 Definition structTy (d:descriptor) : ty :=
   struct_ty_prod (rev (fields d)).
 
+Fixpoint ty_size (t:ty) : nat :=
+  match t with
+  | prodT t1 t2 => ty_size t1 + ty_size t2
+  (* this gives unit values space, which seems fine *)
+  | _ => 1
+  end.
+
+Fixpoint load_ty (t:ty) (e:expr) : expr :=
+  match t with
+  | prodT t1 t2 => (load_ty t1 e, load_ty t2 (e +ₗ #(ty_size t1)))
+  | _ => !e
+  end.
+
+Definition loadStruct (d:descriptor) : val :=
+  λ: "p", load_ty (structTy d) (Var "p").
+
+Fixpoint field_offset (fields: list (string*ty)) f0 : (Z * ty) :=
+  match fields with
+  | nil => (-1, unitT)
+  | f::fs => if String.eqb (fst f) f0 then (0, snd f)
+           else let (off, t) := field_offset fs f0 in
+                (ty_size (snd f) + off, t)
+  end%Z.
+
+Definition loadField (d:descriptor) (f:string) : val :=
+  let (off, t) := field_offset d.(fields) f in
+  λ: "p", load_ty t (Var "p" +ₗ #off).
+
 End go_lang.
 
 Declare Reduction getField := cbv [getField rev fst snd app getField_e fields String.eqb Ascii.eqb eqb].
@@ -87,6 +112,9 @@ Module struct.
   Notation new := mkStruct.
   Notation mk := buildStruct.
   Notation get := getField.
+  (* TODO: load/loadF could probably use better names *)
+  Notation load := loadStruct.
+  Notation loadF := loadField.
   Notation t := structTy.
 End struct.
 
